revert all changes to Pulse.Lib.ArrayPtr.fst

pulse/lib/pulse/lib/Pulse.Lib.ArrayPtr.fst
@@ -18,107 +18,21 @@ module Pulse.Lib.ArrayPtr
 #lang-pulse
 
 noeq
-type base_t ([@@@strictly_positive] a: Type0) =
-| Null
-| Ref of R.ref a
-| Array of A.array a
-
-let base_length
-  (#t: Type)
-  (b: base_t t)
-: GTot nat
-= match b with
-  | Null -> 0
-  | Ref _ -> 1
-  | Array a -> A.length a
-
-noeq
 type ptr t = {
-    base: base_t t;
-    offset: (offset: SZ.t { SZ.v offset <= base_length base})
+    base: A.array u#0 t;
+    offset: (offset: SZ.t { SZ.v offset <= A.length base})
 }
 
 let base a = a.base
 let offset a = SZ.v a.offset
 
-let null #t = { base = Null; offset = 0sz }
-
-let g_is_null p = Null? p.base
-
-let v_is_empty (#t: Type) (s: ptr t) (v: Seq.seq t) : Tot slprop =
-  pure (offset s <= 1 /\ Seq.length v == 0)
-
 let pts_to s #p v =
-  match s.base with
-  | Array a -> A.pts_to_range a (SZ.v s.offset) (SZ.v s.offset + Seq.length v) #p v
-  | Ref a -> if offset s = 0 && Seq.length v = 1 then R.pts_to a #p (Seq.index v 0) else v_is_empty s v
-  | Null -> pure False
-
-ghost fn pts_to_not_null
-  (#t:Type)
-  (s:ptr t)
-  (#p:perm)
-  (#v : Seq.seq t)
-requires
-  (pts_to s #p v)
-ensures
-  (pts_to s #p v ** pure (not (g_is_null s)))
-{
-  if Null? s.base {
-    rewrite (pts_to s #p v) as (pure False);
-    rewrite emp as (pts_to s #p v)
-  } else {
-    ()
-  }
-}
-
-ghost fn pts_to_length
-  (#t:Type)
-  (s:ptr t)
-  (#p:perm)
-  (#v : Seq.seq t)
-requires
-  (pts_to s #p v)
-ensures
-  (pts_to s #p v ** pure (offset s + Seq.length v <= base_length (base s)))
-{
-  pts_to_not_null s;
-  if (Array? s.base) {
-    let Array a = s.base;
-    rewrite pts_to s #p v
-      as A.pts_to_range a (SZ.v s.offset) (SZ.v s.offset + Seq.length v) #p v;
-    A.pts_to_range_prop a;
-    rewrite A.pts_to_range a (SZ.v s.offset) (SZ.v s.offset + Seq.length v) #p v
-      as pts_to s #p v;
-  } else if (s.offset = 0sz && Seq.length v = 1) {
-    ()
-  } else {
-    let Ref a = s.base;
-    rewrite (pts_to s #p v) as (v_is_empty s v);
-    unfold (v_is_empty s v);
-    fold (v_is_empty s v);
-    rewrite (v_is_empty s v) as (pts_to s #p v)
-  }
-}
-
-fn is_null
-  (#t:Type)
-  (s:ptr t)
-  (#p:perm)
-  (#v : Ghost.erased (Seq.seq t))
-requires
-  (pts_to_or_null s #p v)
-returns res: bool
-ensures
-  (pts_to_or_null s #p v ** pure (res == g_is_null s))
-{
-  Null? s.base
-}
+  A.pts_to_range s.base (SZ.v s.offset) (SZ.v s.offset + Seq.length v) #p v
 
 let pts_to_timeless x p s = ()
 
 let is_from_array s sz a =
-    pure (sz == A.length a /\ s.base == Array a)
+    pure (sz == A.length a /\ s.base == a)
 
 fn from_array (#t: Type) (a: A.array t) (#p: perm) (#v: Ghost.erased (Seq.seq t))
     requires A.pts_to a #p v
@@ -127,13 +41,14 @@ fn from_array (#t: Type) (a: A.array t) (#p: perm) (#v: Ghost.erased (Seq.seq t)
 {
     A.pts_to_len a;
     let res = {
-        base = Array a;
+        base = a;
         offset = 0sz;
     };
     fold (is_from_array res (Seq.length v) a);
     A.pts_to_range_intro a p v;
     rewrite (A.pts_to_range a 0 (A.length a) #p v)
-        as (pts_to res #p v);
+        as (A.pts_to_range res.base (SZ.v res.offset) (SZ.v res.offset + Seq.length v) #p v);
+    fold pts_to res #p v;
     res
 }
 
@@ -143,40 +58,11 @@ fn to_array (#t: Type) (s: ptr t) (a: array t) (#p: perm) (#v: Seq.seq t)
     ensures A.pts_to a #p v
 {
     unfold is_from_array s (Seq.length v) a;
-    rewrite (pts_to s #p v)
-      as (A.pts_to_range a (SZ.v s.offset) (SZ.v s.offset + Seq.length v) #p v); 
-    A.pts_to_range_prop a;
-    rewrite (A.pts_to_range a (SZ.v s.offset) (SZ.v s.offset + Seq.length v) #p v)
+    unfold pts_to s #p v;
+    A.pts_to_range_prop s.base;
+    rewrite (A.pts_to_range s.base (SZ.v s.offset) (SZ.v s.offset + Seq.length v) #p v)
         as (A.pts_to_range a 0 (A.length a) #p v);
     A.pts_to_range_elim a _ _;
-}
-
-let is_from_ref s a =
-    pure (s.base == Ref a)
-
-fn from_ref (#t: Type) (a: R.ref t) (#p: perm) (#v: Ghost.erased (t))
-    requires R.pts_to a #p v
-    returns s: ptr t
-    ensures pts_to s #p (Seq.create 1 (Ghost.reveal v)) ** is_from_ref s a
-{
-    let res = {
-        base = Ref a;
-        offset = 0sz;
-    };
-    fold (is_from_ref res a);
-    rewrite (R.pts_to a #p v)
-        as (pts_to res #p (Seq.create 1 (Ghost.reveal v)));
-    res
-}
-
-ghost
-fn to_ref (#t: Type) : to_ref_t t
-= (s: ptr t) (a: ref t) (#p: perm) (#v: Seq.seq t)
-{
-    pts_to_length s;
-    unfold is_from_ref s a;
-    rewrite (pts_to s #p v)
-      as (R.pts_to a #p (Seq.index v 0))
 }
 
 fn op_Array_Access
@@ -194,24 +80,11 @@ fn op_Array_Access
               SZ.v i < Seq.length s /\
               res == Seq.index s (SZ.v i))
 {
-    pts_to_not_null a;
-  if (Array? a.base) {
-    let Array ar = a.base;    
-    rewrite (pts_to a #p s)
-      as (A.pts_to_range ar (SZ.v a.offset) (SZ.v a.offset + Seq.length s) #p s); 
-    A.pts_to_range_prop ar;
-    let res = A.pts_to_range_index ar (SZ.add a.offset i);
-    rewrite (A.pts_to_range ar (SZ.v a.offset) (SZ.v a.offset + Seq.length s) #p s)
-      as (pts_to a #p s);
+    unfold pts_to a #p s;
+    A.pts_to_range_prop a.base;
+    let res = A.pts_to_range_index a.base (SZ.add a.offset i);
+    fold pts_to a #p s;
     res
-  } else {
-    pts_to_length a;
-    let Ref r = a.base;
-    rewrite (pts_to a #p s) as (R.pts_to r #p (Seq.index s 0));
-    let res = !r;
-    rewrite (R.pts_to r #p (Seq.index s 0)) as (pts_to a #p s);
-    res
-  }
 }
 
 fn op_Array_Assignment
@@ -228,25 +101,15 @@ fn op_Array_Assignment
               s' == Seq.upd s (SZ.v i) v
             )
 {
-    pts_to_not_null a;
-  if (Array? a.base) {
-    let Array ar = a.base;
-    rewrite (pts_to a s)
-      as (A.pts_to_range ar (SZ.v a.offset) (SZ.v a.offset + Seq.length s) s);
-    A.pts_to_range_prop ar;
-    let res = A.pts_to_range_upd ar (SZ.add a.offset i) v;
+    unfold pts_to a s;
+    A.pts_to_range_prop a.base;
+    let res = A.pts_to_range_upd a.base (SZ.add a.offset i) v;
     rewrite
-      A.pts_to_range ar (SZ.v a.offset) (SZ.v a.offset + Seq.length s) (Seq.upd s (SZ.v i) v)
+      A.pts_to_range a.base (SZ.v a.offset) (SZ.v a.offset + Seq.length s) (Seq.upd s (SZ.v i) v)
     as
-      pts_to a (Seq.upd s (SZ.v i) v);
+      A.pts_to_range a.base (SZ.v a.offset) (SZ.v a.offset + Seq.length (Seq.upd s (SZ.v i) v)) (Seq.upd s (SZ.v i) v);
+    fold pts_to a (Seq.upd s (SZ.v i) v);
     ();
-  } else {
-    pts_to_length a;
-    let Ref r = a.base;
-    rewrite (pts_to a s) as (R.pts_to r (Seq.index s 0));
-    r := v;
-    rewrite (R.pts_to r v) as (pts_to a (Seq.upd s (SZ.v i) v));
-  }
 }
 
 ghost
@@ -258,39 +121,10 @@ fn share
   requires pts_to arr #p s
   ensures pts_to arr #(p /. 2.0R) s ** pts_to arr #(p /. 2.0R) s
 {
-    pts_to_not_null arr;
-  if (Array? arr.base) {
-    let Array a = arr.base;
-    rewrite (pts_to arr #p s)
-      as (A.pts_to_range a (SZ.v arr.offset) (SZ.v arr.offset + Seq.length s) #p s);
-    A.pts_to_range_share a;
-    rewrite (A.pts_to_range a (SZ.v arr.offset) (SZ.v arr.offset + Seq.length s) #(p /. 2.0R) s)
-      as (pts_to arr #(p /. 2.0R) s);
-    rewrite (A.pts_to_range a (SZ.v arr.offset) (SZ.v arr.offset + Seq.length s) #(p /. 2.0R) s)
-      as (pts_to arr #(p /. 2.0R) s);
-  } else {
-    let test = (offset arr = 0 && Seq.length (Ghost.reveal s) = 1);
-    if (test) {
-      let Ref a = arr.base;
-      rewrite (pts_to arr #p s)
-        as (R.pts_to a #p (Seq.index s 0));
-      R.share a;
-      rewrite (R.pts_to a #(p /. 2.0R) (Seq.index s 0))
-        as (pts_to arr #(p /. 2.0R) s);
-      rewrite (R.pts_to a #(p /. 2.0R) (Seq.index s 0))
-        as (pts_to arr #(p /. 2.0R) s);
-    } else {
-      rewrite (pts_to arr #p s)
-        as (v_is_empty arr s);
-      unfold (v_is_empty arr s);
-      fold (v_is_empty arr s);
-      rewrite (v_is_empty arr s)
-        as (pts_to arr #(p /. 2.0R) s);
-      fold (v_is_empty arr s);
-      rewrite (v_is_empty arr s)
-        as (pts_to arr #(p /. 2.0R) s);
-    }
-  }
+    unfold pts_to arr #p s;
+    A.pts_to_range_share arr.base;
+    fold pts_to arr #(p /. 2.0R) s;
+    fold pts_to arr #(p /. 2.0R) s;
 }
 
 ghost
@@ -302,99 +136,11 @@ fn gather
   requires pts_to arr #p0 s0 ** pts_to arr #p1 s1 ** pure (Seq.length s0 == Seq.length s1)
   ensures pts_to arr #(p0 +. p1) s0 ** pure (s0 == s1)
 {
-    pts_to_not_null arr #p0;
-  if (Array? arr.base) {
-    let Array a = arr.base;
-    rewrite (pts_to arr #p0 s0)
-      as (A.pts_to_range a (SZ.v arr.offset) (SZ.v arr.offset + Seq.length s0) #(p0) s0);
-    rewrite pts_to arr #p1 s1
-      as (A.pts_to_range a (SZ.v arr.offset) (SZ.v arr.offset + Seq.length s0) #(p1) s1);
-    A.pts_to_range_gather a #_ #_ #s0 #s1 #p0 #p1;
-    rewrite (A.pts_to_range a (SZ.v arr.offset) (SZ.v arr.offset + Seq.length s0) #(p0 +. p1) s0)
-      as pts_to arr #(p0 +. p1) s0
-  } else {
-    let test = (offset arr = 0 && Seq.length (Ghost.reveal s0) = 1);
-    if (test) {
-      let Ref a = arr.base;
-      rewrite (pts_to arr #p0 s0)
-        as (R.pts_to a #p0 (Seq.index s0 0));
-      rewrite (pts_to arr #p1 s1)
-        as (R.pts_to a #p1 (Seq.index s1 0));
-      R.gather a;
-      assert (pure (Seq.equal s0 s1));
-      rewrite (R.pts_to a #(p0 +. p1) (Seq.index s0 0))
-        as (pts_to arr #(p0 +. p1) s0);
-    } else {
-      rewrite (pts_to arr #p0 s0)
-        as (v_is_empty arr s0);
-      unfold (v_is_empty arr s0);
-      rewrite (pts_to arr #p1 s1)
-        as (v_is_empty arr s1);
-      unfold (v_is_empty arr s1);
-      assert (pure (Seq.equal s0 s1));
-      fold (v_is_empty arr s0);
-      rewrite (v_is_empty arr s0)
-        as (pts_to arr #(p0 +. p1) s0);
-    }
-  }
-}
-
-let shift
-  (#t: Type) (s: ptr t) (i: SZ.t { SZ.v s.offset + SZ.v i <= base_length s.base })
-: Tot (ptr t)
-= 
-  {
-        base = s.base;
-        offset = SZ.add s.offset i;
-  }
-
-ghost fn ghost_shift (#t: Type) (s: ptr t) (#p: perm) (i: SZ.t)
-    (#v: Ghost.erased (Seq.seq t) { SZ.v i <= Seq.length v })
-  requires pts_to s #p v
-  returns res: squash (SZ.v s.offset + SZ.v i <= base_length s.base)
-  ensures
-    pts_to s #p (Seq.slice v 0 (SZ.v i)) **
-    pts_to (shift s i) #p (Seq.slice v (SZ.v i) (Seq.length v))
-{
-    pts_to_not_null s;
-  if (Array? s.base) {
-    let Array a = s.base;
-    rewrite pts_to s #p v
-      as A.pts_to_range a (SZ.v s.offset) (SZ.v s.offset + Seq.length v) #p v;
-    A.pts_to_range_prop a;
-    let s' = shift s i;
-    A.pts_to_range_split a _ (SZ.v s'.offset) _;
-    with s1. assert A.pts_to_range a (SZ.v s.offset) (SZ.v s'.offset) #p s1;
-    rewrite
-        (A.pts_to_range a (SZ.v s.offset) (SZ.v s'.offset) #p s1)
-        as pts_to s #p s1;
-    with s2. assert A.pts_to_range a (SZ.v s'.offset) (SZ.v s.offset + Seq.length v) #p s2;
-    rewrite
-        (A.pts_to_range a (SZ.v s'.offset) (SZ.v s.offset + Seq.length v) #p s2)
-        as pts_to (shift s i) #p s2;
-    ()
-  } else {
-    pts_to_length s;
-    let res : squash (SZ.v s.offset + SZ.v i <= base_length s.base) = ();
-    let Ref a = s.base;
-    let test = (SZ.v i + 1 <= Seq.length v);
-    if (test) {
-      assert (pure (Seq.equal v (Seq.slice v (SZ.v i) (Seq.length v))));
-      rewrite pts_to s #p v
-        as pts_to (shift s i) #p (Seq.slice v (SZ.v i) (Seq.length v));
-      fold (v_is_empty s (Seq.slice v 0 (SZ.v i)));
-      rewrite (v_is_empty s (Seq.slice v 0 (SZ.v i)))
-        as pts_to s #p (Seq.slice v 0 (SZ.v i));
-    } else {
-      assert (pure (Seq.equal v (Seq.slice v 0 (SZ.v i))));
-      rewrite pts_to s #p v
-        as pts_to s #p (Seq.slice v 0 (SZ.v i));
-      fold (v_is_empty s (Seq.slice v (SZ.v i) (Seq.length v)));
-      rewrite (v_is_empty s (Seq.slice v (SZ.v i) (Seq.length v)))
-        as pts_to (shift s i) #p (Seq.slice v (SZ.v i) (Seq.length v));
-      res
-    }
-  }
+    unfold pts_to arr #p0 s0;
+    unfold pts_to arr #p1 s1;
+    rewrite each Seq.length s1 as Seq.length s0;
+    A.pts_to_range_gather arr.base #_ #_ #s0 #s1 #p0 #p1;
+    fold pts_to arr #(p0 +. p1) s0
 }
 
 fn split (#t: Type) (s: ptr t) (#p: perm) (i: SZ.t)
@@ -406,8 +152,24 @@ fn split (#t: Type) (s: ptr t) (#p: perm) (i: SZ.t)
     pts_to s' #p (Seq.slice v (SZ.v i) (Seq.length v)) **
     pure (adjacent s (SZ.v i) s')
 {
-    ghost_shift s i;
-    shift s i
+    unfold pts_to s #p v;
+    A.pts_to_range_prop s.base;
+    let s' = {
+        base = s.base;
+        offset = SZ.add s.offset i;
+    };
+    A.pts_to_range_split s.base _ (SZ.v s'.offset) _;
+    with s1. assert A.pts_to_range s.base (SZ.v s.offset) (SZ.v s'.offset) #p s1;
+    rewrite
+        (A.pts_to_range s.base (SZ.v s.offset) (SZ.v s'.offset) #p s1)
+        as (A.pts_to_range s.base (SZ.v s.offset) (SZ.v s.offset + Seq.length s1) #p s1);
+    fold pts_to s #p s1;
+    with s2. assert A.pts_to_range s.base (SZ.v s'.offset) (SZ.v s.offset + Seq.length v) #p s2;
+    rewrite
+        (A.pts_to_range s.base (SZ.v s'.offset) (SZ.v s.offset + Seq.length v) #p s2)
+        as (A.pts_to_range s'.base (SZ.v s'.offset) (SZ.v s'.offset + Seq.length s2) #p s2);
+    fold pts_to s' #p s2;
+    s'
 }
 
 ghost fn ghost_split (#t: Type) (s: ptr t) (#p: perm) (i: SZ.t)
@@ -419,8 +181,24 @@ ghost fn ghost_split (#t: Type) (s: ptr t) (#p: perm) (i: SZ.t)
     pts_to (reveal s') #p (Seq.slice v (SZ.v i) (Seq.length v)) **
     pure (adjacent s (SZ.v i) s')
 {
-    ghost_shift s i;
-    shift s i
+    unfold pts_to s #p v;
+    A.pts_to_range_prop s.base;
+    let s' = {
+        base = s.base;
+        offset = SZ.add s.offset i;
+    };
+    A.pts_to_range_split s.base _ (SZ.v s'.offset) _;
+    with s1. assert A.pts_to_range s.base (SZ.v s.offset) (SZ.v s'.offset) #p s1;
+    rewrite
+        (A.pts_to_range s.base (SZ.v s.offset) (SZ.v s'.offset) #p s1)
+        as (A.pts_to_range s.base (SZ.v s.offset) (SZ.v s.offset + Seq.length s1) #p s1);
+    fold pts_to s #p s1;
+    with s2. assert A.pts_to_range s.base (SZ.v s'.offset) (SZ.v s.offset + Seq.length v) #p s2;
+    rewrite
+        (A.pts_to_range s.base (SZ.v s'.offset) (SZ.v s.offset + Seq.length v) #p s2)
+        as (A.pts_to_range s'.base (SZ.v s'.offset) (SZ.v s'.offset + Seq.length s2) #p s2);
+    fold pts_to s' #p s2;
+    s'
 }
 
 
@@ -429,33 +207,15 @@ fn join (#t: Type) (s1: ptr t) (#p: perm) (#v1: Seq.seq t) (s2: ptr t) (#v2: Seq
     requires pts_to s1 #p v1 ** pts_to s2 #p v2 ** pure (adjacent s1 (Seq.length v1) s2)
     ensures pts_to s1 #p (Seq.append v1 v2)
 {
-    pts_to_not_null s1;
-  if (Array? s1.base) {
-    let Array a = s1.base;
-    rewrite pts_to s1 #p v1
-      as (A.pts_to_range a (SZ.v s1.offset) (SZ.v s1.offset + Seq.length v1) #p v1);
-    rewrite pts_to s2 #p v2
-        as (A.pts_to_range a (SZ.v s1.offset + Seq.length v1) (SZ.v s1.offset + Seq.length v1 + Seq.length v2) #p v2);
-    A.pts_to_range_join a (SZ.v s1.offset) (SZ.v s1.offset + Seq.length v1) (SZ.v s1.offset + Seq.length v1 + Seq.length v2);
-    rewrite (A.pts_to_range a (SZ.v s1.offset) (SZ.v s1.offset + Seq.length v1 + Seq.length v2) #p (Seq.append v1 v2))
-    as pts_to s1 #p (Seq.append v1 v2)
-  } else {
-    pts_to_length s1;
-    pts_to_length s2;
-    if (Seq.length v2 = 0) {
-      rewrite pts_to s2 #p v2 as v_is_empty s2 v2;
-      unfold v_is_empty s2 v2;
-      assert (pure (Seq.equal v1 (Seq.append v1 v2)));
-      rewrite pts_to s1 #p v1 as pts_to s1 #p (Seq.append v1 v2);
-    } else {
-      let Ref a = s1.base;
-      rewrite pts_to s1 #p v1 as v_is_empty s1 v1;
-      unfold v_is_empty s1 v1;
-      assert (pure (Seq.equal v2 (Seq.append v1 v2)));
-      rewrite pts_to s2 #p v2 as pts_to s1 #p (Seq.append v1 v2);
-    }
-  }
+    unfold pts_to s1 #p v1;
+    unfold pts_to s2 #p v2;
+    rewrite (A.pts_to_range s2.base (SZ.v s2.offset) (SZ.v s2.offset + Seq.length v2) #p v2)
+        as (A.pts_to_range s1.base (SZ.v s1.offset + Seq.length v1) (SZ.v s1.offset + Seq.length (Seq.append v1 v2)) #p v2);
+    A.pts_to_range_join s1.base (SZ.v s1.offset) (SZ.v s1.offset + Seq.length v1) (SZ.v s1.offset + Seq.length (Seq.append v1 v2));
+    fold pts_to s1 #p (Seq.append v1 v2)
 }
+
+module R = Pulse.Lib.Reference
 
 fn memcpy
     (#t:Type0) (#p0:perm)
